Bring up to date with CompCert trunk

compcert/cfrontend/Clight.v
@@ -600,7 +600,6 @@ Inductive step: state -> trace -> state -> Prop :=
         E0 (Returnstate v' (call_cont k) m')
   | step_skip_call: forall f k e le m m',
       is_call_cont k ->
-      f.(fn_return) = Tvoid ->
       Mem.free_list m (blocks_of_env e) = Some m' ->
       step (State f Sskip k e le m)
         E0 (Returnstate Vundef k m')
